Comments, test, and a new well_formed predicate

test/LinkedList.fst
@@ -85,11 +85,16 @@ let rec list_is_live #a #n (h: HS.mem) (l: t a {list_has_length h l n}):
       cell_is_live h l /\
       list_is_live #a #(n - 1) h next
 
+/// Thus, a well-formed list is both paired with a predicate for its length, and
+/// states that are the list cells are live in the current heap.
+let well_formed #a (h: HS.mem) (l: t a) (n: nat) =
+  list_has_length h l n /\ list_is_live #a #n h l
+
 /// This form will rarely turn out to be useful, except perhaps for user code.
 /// Indeed, we most often want to tie the length of the list in the final state
 /// with its length in the original state.
 let live #a (h: HS.mem) (l: t a) =
-  exists n. list_has_length h l n /\ list_is_live #a #n h l
+  exists n. well_formed #a h l n
 
 
 /// As we start proving some degree of functional correctness, we will have to
@@ -97,60 +102,35 @@ let live #a (h: HS.mem) (l: t a) =
 /// the footprint of a given list.
 /// TODO: proper patterns for quantifiers!
 #set-options "--max_ifuel 0 --max_fuel 1"
-val footprint: (#a: Type) -> (#n: nat) -> (h: HS.mem) -> (l: t a) -> Ghost (list (ref (cell a)))
-  (requires (
-    list_has_length h l n /\
-    list_is_live #a #n h l
-  ))
+val footprint: (#a: Type) -> (h: HS.mem) -> (l: t a) -> (n: nat) -> Ghost (list (ref (cell a)))
+  (requires (well_formed h l n))
   (ensures (fun refs ->
     let n_refs = L.length refs in
     n_refs = n /\
-    (forall (i: nat). i < n ==>
-      list_has_length h (L.index refs (n - 1 - i)) (i + 1) /\
-      cell_is_live #a h (L.index refs (n - 1 - i)))
-  ))
+    (forall (i: nat). i < n ==> well_formed h (L.index refs (n - 1 - i)) (i + 1))))
+  (decreases n)
 
-let rec footprint #a #n h l =
+let rec footprint #a h l n =
   match HS.sel h l with
   | Nil ->
       []
   | Cons next _ ->
-      let refs = footprint #a #(n - 1) h next in
+      let refs = footprint h next (n - 1) in
       l :: refs
 #reset-options
-
-/// An intermediary lemma, for sanity (it is currently unused): the head is
-/// disjoint from anything found in the footprint of the tail. The
-/// list_has_length predicate provides an easy contradiction if it were the
-/// case.
-/// TODO: pattern!
-let list_next_disjoint_i (#a: Type) (#n: nat) (h: HS.mem) (l: t a) (i: nat):
-  Lemma
-    (requires (
-      list_has_length h l n /\
-      list_is_live #a #n h l /\
-      i < n - 1 /\
-      Cons? (HS.sel h l)))
-    (ensures (
-      let next = Cons?.next (HS.sel h l) in
-      let refs = footprint #a #(n - 1) h next in
-      HS.as_addr l <> HS.as_addr (L.index refs i)
-    ))
-=
-  ()
 
 /// All the reasoning about the pop operation is done in this lemma. If `head`
 /// is not found in the footprint of `l`, then the specific write we perform for
 /// pop (we could be more generic!) leaves the two essential predicates
 /// untouched for l.
-val pop_preserves_live: (#a: Type) -> (#n: nat) -> (h0: HS.mem) -> (head: ref (cell a)) -> (l: t a) ->
+/// TODO: this proof is slow / investigate
+val pop_preserves_live: (#a: Type) -> (h0: HS.mem) -> (head: ref (cell a)) -> (l: t a) -> (n: nat) ->
   Lemma
     (requires (
       live h0 head /\
       Cons? (HS.sel h0 head) /\
-      list_has_length h0 l n /\
-      list_is_live #a #n h0 l /\ (
-      let refs = footprint #a #n h0 l in
+      well_formed h0 l n /\ (
+      let refs = footprint h0 l n in
       forall (i: nat). i < n ==> HS.as_addr head <> HS.as_addr (L.index refs i)
     )))
     (ensures (
@@ -158,26 +138,31 @@ val pop_preserves_live: (#a: Type) -> (#n: nat) -> (h0: HS.mem) -> (head: ref (c
       Cons? (HS.sel h0 head) /\ (
       let next = Cons?.next (HS.sel h0 head) in
       let h1 = HS.upd h0 head (HS.sel h0 next) in
-      list_has_length h1 l n /\
-      list_is_live #a #n h1 l
+      well_formed h1 l n
     )))
     (decreases n)
-    [ SMTPat (list_is_live #a #n h0 l); SMTPat (Cons? (HS.sel h0 head)) ]
+    [ SMTPat (well_formed #a h0 l n); SMTPat (Cons? (HS.sel h0 head)) ]
 
 #set-options "--z3rlimit 40 --max_ifuel 0"
-let rec pop_preserves_live #a #n h0 head l =
+let rec pop_preserves_live #a h0 head l n =
   match HS.sel h0 l with
   | Nil -> ()
   | Cons l' _ ->
-      pop_preserves_live #a #(n - 1) h0 head l'
+      pop_preserves_live h0 head l' (n - 1)
 
+/// Finally, the pop operation. The code is straightforward and crucially relies
+/// on the call to the lemma above. Note that at this stage we do not prove full
+/// functional correctness of our implementation. Rather, we just state that the
+/// lengths is as expected.
+/// TODO: move this code to use an erased integer... but merely computing n - 1
+/// below behind an erased type is tedious.
 val pop: (#a: Type) -> (#n: nat) -> (l: t a) ->
   ST (option a)
-  (requires (fun h -> list_has_length h l n /\ list_is_live #a #n h l))
+  (requires (fun h -> well_formed h l n))
   (ensures (fun h0 v h1 ->
     match v with
-    | None -> list_has_length h1 l n /\ list_is_live #a #n h1 l
-    | Some _ -> n > 0 /\ list_has_length h1 l (n - 1) /\ list_is_live #a #(n - 1) h1 l
+    | None -> n = 0 /\ well_formed h1 l n
+    | Some _ -> n > 0 /\ well_formed h1 l (n - 1)
   ))
 
 let pop #a #n l =
@@ -186,5 +171,13 @@ let pop #a #n l =
   | Cons next data ->
       let h0 = get () in
       l := !next;
-      pop_preserves_live #a #(n - 1) h0 l next;
+      pop_preserves_live #a h0 l next (n - 1);
       Some data
+
+/// Purely a test function to see some actual code.
+let test_pop #n (l: t UInt32.t): ST UInt32.t
+  (requires (fun h -> well_formed h l n))
+  (ensures (fun _ _ _ -> true)) =
+  match pop #UInt32.t #n l with
+  | None -> 0ul
+  | Some x -> x
